tests/lean/run/liaByRefl.lean
@@ -74,14 +74,12 @@ example (x₁ x₂ x₃ : Int) : ((x₁ + x₂) + (x₂ + x₃) = x₃ + x₂) =
   RawRelCnstr.eq_of_norm_eq #R[x₁, x₂, x₃]
     (.eq (Expr.add (Expr.add (Expr.var 0) (Expr.var 1)) (Expr.add (Expr.var 1) (Expr.var 2)))
          (Expr.add (Expr.var 2) (Expr.var 1)))
-    (.eq (Expr.add (Expr.var 0) (Expr.var 1))
-         (Expr.num 0))
+    (.eq (.add 1 0 (.add 1 1 (.num 0))))
     rfl
 
 example (x₁ x₂ x₃ : Int) : ((x₁ + x₂) + (x₂ + x₃) ≤ x₃ + x₂) = (x₁ + x₂ ≤ 0) :=
   RawRelCnstr.eq_of_norm_eq #R[x₁, x₂, x₃]
     (.le (Expr.add (Expr.add (Expr.var 0) (Expr.var 1)) (Expr.add (Expr.var 1) (Expr.var 2)))
          (Expr.add (Expr.var 2) (Expr.var 1)))
-    (.le (Expr.add (Expr.var 0) (Expr.var 1))
-         (Expr.num 0))
+    (.le (Poly.add 1 0 (.add 1 1 (.num 0))))
     rfl
